VerificationSetCover_contador_simple.dfy
@@ -13,32 +13,42 @@ ensures exists s :: s in S && maximumSizeElements(S) == |s|
 
 // * LA TRANSFORMACIÓN DE SET COVER ES POLINÓMICA
 
-method HittingSet_to_SetCover_Method(U: set<int>, S: set<set<int>>, k: nat) returns (r:(set<set<int>>, set<set<set<int>>>, int))
+method HittingSet_to_SetCover_Method(U: set<int>, S: set<set<int>>, k: nat) returns (r:(set<set<int>>, set<set<set<int>>>, int), counter:int)
   requires forall s | s in S ::  s <= U
   //ensures forall s | s in r.1 :: s <= r.0
   //ensures isCover(r.0, r.1)
   {
+    counter := 0;
     //var newS: set<set<set<int>>> := (set u | u in U :: (set s | s in S && u in s));
     var newS:set<set<set<int>>> := {};
     var U' := U;
+    counter := counter + |U|;
+
+    counter := counter + 1;
+
     while (U' != {})
     {
       var u :| u in U';
       U' := U' - {u};
+      counter := counter + |U|;
 
       var sets_in_S_that_contain_u:set<set<int>> := {};
       var S' := S;
+      counter := counter + |S|*|U|;
       while (S' != {}) {
         var s :| s in S';
         S' := S' - {s};
+        counter := counter + |S|*|U|;
 
         if (u in s) {
           sets_in_S_that_contain_u := sets_in_S_that_contain_u + {s};
         }
-
       }
 
       newS := newS + {sets_in_S_that_contain_u};
+      counter := counter + |S|*|U|;
+
+      counter := counter + 1;
     }
 
 
@@ -59,10 +69,10 @@ method HittingSet_to_SetCover_Method(U: set<int>, S: set<set<int>>, k: nat) retu
     (S, newS, k)
     */
     if (S_contains_empty) {
-
+      // ...
     }
     else {
-      return (S, newS, k);
+      return (S, newS, k), counter;
     }
 
     assume false;
